refactor stateT and writerT monads to use the definitions in extlib.

theories/Events/Map.v
@@ -9,6 +9,9 @@ Import ListNotations.
 
 From ExtLib.Structures Require Maps.
 
+From ExtLib Require Import
+     Data.Monads.StateMonad.
+
 From ITree Require Import
      Basics.Basics
      Basics.CategoryOps
@@ -19,7 +22,6 @@ From ITree Require Import
      Interp.Interp
      Events.State.
 
-Import ITree.Basics.Basics.Monads.
 (* end hide *)
 
 Section Map.
@@ -50,15 +52,17 @@ Section Map.
   Context {M : Map K V map}.
 
   Definition handle_map {E} : mapE ~> stateT map (itree E) :=
-    fun _ e env =>
+    fun _ e =>
       match e with
-      | Insert k v => Ret (Maps.add k v env, tt)
-      | Lookup k => Ret (env, Maps.lookup k env)
-      | Remove k => Ret (Maps.remove k env, tt)
+      | Insert k v => mkStateT (fun env => Ret (tt, Maps.add k v env))
+      | Lookup k => mkStateT (fun env => Ret (Maps.lookup k env, env))
+      | Remove k => mkStateT (fun env => Ret (tt, Maps.remove k env))
       end.
 
+  (* not sure why case_ requires manual parameters *)
   Definition run_map {E} : itree (mapE +' E) ~> stateT map (itree E) :=
-    interp_state (case_ handle_map pure_state).
+    interp_state (case_ (bif := sum1) (c := stateT map (itree E))
+                        handle_map pure_state).
 
 End Map.
 
